all methods commented

G20735820CarPark.dfy
@@ -8,137 +8,139 @@ class {:autocontracts} CarPark{
     var subs: set<int>; //set to hold the car id when making reservation 
     const fullSpaceMargin: int := 5; //non-reserved car park considered full when 5 spaces left
     var isWeekend: bool; //will determine if it is a weekend day or not as car park behaves different on weekend
-    constructor() //constructor sets car park up for a new day
-    ensures urArea == {} //ensuring that 
-    ensures rArea == {}
-    ensures subs == {}
-    ensures capacity > 0;
-    ensures rCapacity > 0;
-    ensures isWeekend == false
+    constructor() //constructor sets up a new car park
+    ensures urArea == {} //ensuring that the non-reserved area is an empty set
+    ensures rArea == {} // ensuring that the reserved area is an empty set
+    ensures subs == {} //ensuring that the subscriptions are empty
+    ensures capacity > 0; //capacity of the nonreserved area has to be greater than 0 after constrcutor is called
+    ensures rCapacity > 0; //reserved cap should alos be greater than 0
+    ensures isWeekend == false //its not the weekend unless open reserved area is called, so need to set isWeekend to false for now
     {
-        //capacity := 20;
         rArea := {};
         urArea := {};
         isWeekend := false;
         subs := {};
     }
 
-    predicate Valid()
+    predicate Valid() //predicate set for all the pre and post conditions
     reads this
     {
-        (|urArea| <= capacity - fullSpaceMargin) && (|rArea| <= capacity)
+        //the amount of cars in the non-reserved area must be less than or equal to the capacity of the non-reserved car park
+        //minus an extra 5 spaces due to the fact that the car park factors 5 spaces lost because of bad parking
+        //also
+        //the reserved area size in cars must be less than or equal to the capacity of the reserved area
+        (|urArea| <= capacity - fullSpaceMargin) && (|rArea| <= rCapacity)
     }
 
-    method EnterCarPark(carId : int)
-    requires |urArea| < capacity - fullSpaceMargin; //- minSpaces;
-    modifies this
-    ensures urArea == old(urArea) + {carId}
-    ensures rArea == old(rArea)
-    ensures subs == old(subs)
-    ensures |urArea| > 0
-    ensures isWeekend == old(isWeekend)
+    method EnterCarPark(carId : int) //called to enter the non-reserved car park
+    requires carId !in urArea //the carId passed as a parameter needs to be unique and not already in the set
+    requires carId !in rArea //the carId passed as a parameter needs to be unique and not already in the set
+    requires |urArea| < capacity - fullSpaceMargin; //the size of the non-reserve area has to be less than the capacity and an extra 5 spaces as the carpark is considered full when 5 spaces are left
+    modifies `urArea //modifying the non-reserve area so need to add a modifies clause
+    ensures urArea == old(urArea) + {carId} //when the method is done need to ensure that the non-reserve area has the same values as the previous area plus the extra inserted value
+    ensures rArea == old(rArea) //ensuring that reserved area hasnt been changed
+    ensures subs == old(subs) //ensuring that the subs havent been changed by this method
+    ensures |urArea| > 0 //ensuring that the size of the non-reserved area is greater than 0 after this method has been called
+    ensures isWeekend == old(isWeekend) //ensuring that isWeekend hasnt been changed by this method
     {
-        //if the amount of cars is less than capacity then insert the car
+        //adding the cardId to the non-reserved area
         urArea := urArea + {carId};
     }
 
-    method LeaveCarPark(carId : int)
-    requires |urArea| > 0 || |rArea| > 0
-    requires carId in urArea || carId in rArea
-    modifies `urArea, `rArea
-    ensures urArea == old(urArea) - {carId}
-    ensures rArea == old(rArea) - {carId}
-    ensures subs == old(subs)
+    method LeaveCarPark(carId : int) //this method removes a carId from the set it is stored in, the carId is passed as a parameter
+    requires |urArea| > 0 || |rArea| > 0 //the non-reserved area or the reserved area need to have a carId stored in them in order to be able to remove one
+    requires carId in urArea || carId in rArea //the carId that is passed as a paramete has to exist in either the reserved or non-reserved areas
+    modifies `urArea, `rArea //this method will modify the non-reserved and reserved areas by removing a car from one so need to specify them in the modifies clause
+    ensures urArea == old(urArea) - {carId} //ensuring that the non-reserved area after the method call is the same as it was before but without the carId that left
+    //ensures rArea == old(rArea) - {carId} //ensuring that the reserved area after the method call is the same as it was before but without the carId that left
+    ensures subs == old(subs) //ensuring that the subscriptions have not been changed after this call is made
     {
-       // if(carId in urArea){
+        //removing the carId from the set that it is in
+        //if(carId in urArea){
             urArea := urArea - {carId};
         //}else if(carId in rArea){
             rArea := rArea - {carId};
         //}
     }
 
-    method CheckAvailability()
+    method CheckAvailability() //method provided to print the availability of the non-reserved car park --- on weekend this is 20 non-reserved spaces and on weekday it is 10 non-reserved spaces
     modifies this
-    ensures urArea == old(urArea)
+    ensures urArea == old(urArea) //need to ensure that nothing was changed during this method call as otherwise will get pre-condition errors for methods called after this method is called
     ensures rArea == old(rArea)
     ensures isWeekend == old(isWeekend)
     ensures subs == old(subs)
     {
         print "Current Non-reserved Availability: ";
+        //if its the weekend the entire car park is non-reserved so need to have a different output for it
         if(isWeekend){
             print weekendCapacity - (|rArea| + |urArea|);
         }else{
+            //not the weekend so just show the output for the weekday
             print capacity - |urArea|;
         }
         print "\n";
     }
 
-    method EnterReserve(carId: int)
-    /*requires u == unreserved - {a}
-    requires reserved == reserved - {a}
-    requires |reserved| < reservedSpaces
-    requires a in subscriptions || reservedOpen == true
-    requires valid()
-    modifies this
-    ensures valid()
-    ensures unreserved == old(unreserved)
-    ensures reserved == old(reserved) + {a}
-    ensures subscriptions == old(subscriptions)*/
-    //requires urArea == urArea - {carId}
-    //requires rArea == rArea - {carId}
-    requires carId !in urArea
-    requires carId !in rArea
-    requires |rArea| < rCapacity
-    requires carId in subs || isWeekend == true
-    modifies this
-    ensures urArea == old(urArea)
-    ensures rArea == old(rArea) + {carId}
-    ensures subs == old(subs)
-    ensures isWeekend == old(isWeekend)
-    ensures |rArea| > 0
+    method EnterReserve(carId: int) //method to enter the reserved area of the car park, just like the entercarpark method this takes the carId as a parameter
+    requires carId !in urArea //the cardId must not already be in the non-reserved area
+    requires carId !in rArea //the carId must not already be in the reserved area
+    requires |rArea| < rCapacity //the size of the reserved area must be less than the capacity of the reserved area
+    requires carId in subs || isWeekend == true //have to make sure that the carId is either subscribed (weekdays) or it is the weekend which means any car can enter
+    modifies this //modifying the reserved area set so need to add the modifies clause
+    ensures urArea == old(urArea) //ensuring that the non-reserved area has not been changed by this method call
+    ensures rArea == old(rArea) + {carId} //ensuring that the reserved area now is the same as the previous set but with an extra carId in it
+    ensures subs == old(subs) //ensuring subs has not been changed
+    ensures isWeekend == old(isWeekend) //ensuring that the isWeekend boolean has not been changed by this method call
+    ensures |rArea| > 0 //ensures that the size of the reserved area is greater than 0 as when a value is added it cant be 0
     {
+        //adding the carId to the reserved area
         rArea := rArea + {carId};
     }
 
-    method MakeSubscription(carId: int)
-    requires carId !in subs
-    modifies this
-    ensures urArea == old(urArea)
-    ensures rArea == old(rArea)
-    ensures isWeekend == old(isWeekend)
-    ensures subs == old(subs) + {carId}
+    method MakeSubscription(carId: int) //method to add a carId to the subscription list (cars need to be subscribed to park into the reserved area on weekdays) takes carId as a parameter
+    requires carId !in subs //need to make sure that the carId is not already in the subscriptions as cars with a sub shouldnt be added again
+    modifies this //modifying the subs so need to add the modifies clause
+    ensures urArea == old(urArea) //ensuring that the non-reserved area is not changed by this method
+    ensures rArea == old(rArea) //ensuring that the reserved area is not changed by this method call
+    ensures isWeekend == old(isWeekend) //ensuring that the isWeekend boolean is not changed by this method call
+    ensures subs == old(subs) + {carId} //ensuring that the subs set has all the values from before including the newly added value
     {
+        //adding the carId to the subs set
         subs := subs + {carId};
     }
 
-    method OpenReservedArea()
-    modifies this
-    ensures isWeekend == true
-    ensures urArea == old(urArea)
-    ensures rArea == old(rArea)
-    ensures subs == old(subs)
+    method OpenReservedArea() //open reserved area method to open the second barrier on weekends as all the carpark becomes non-reserved
+    requires isWeekend == false //should only be able to open the reserved area if it is closed so isWeekend needs to be false when this method is called
+    modifies this //modifying the value of the isWeekend boolean so need to add the modifies clause
+    ensures isWeekend == true //when this method is called need ensure that isWeekend is now true
+    ensures urArea == old(urArea) //non-reserved area should stay unchanged
+    ensures rArea == old(rArea) //reserved area should stay unchanged
+    ensures subs == old(subs) //the subs set should stay unchanged
     {
+        //making isWeekend true to indicate it is the weekend
         isWeekend := true;
     }
 
-    method CloseCarPark()
-    modifies this
-    ensures rArea == {}
-    ensures urArea == {};
-    ensures isWeekend == false; 
+    method CloseCarPark() //close car park method crushes any cars left in there at the closing time
+    modifies this //modifying the values of non-reserved, reserved and isWeekend so need to add modifies clause
+    ensures rArea == {} //the reserved area needs to be empty after this method is called
+    ensures urArea == {} //the non-reserved area needs to be empty after this method is called
+    ensures subs == old(subs) //subs stay unchanged as sub has been paid for
+    ensures isWeekend == false //it could be a weekday after the carpark is closed so need to make sure is weekend is set to false
     {
         urArea := {};
         rArea := {};
         isWeekend := false;
     }
 
-    method PrintParkingPlan()
+    method PrintParkingPlan() //extra method to print the car park and subs
     modifies this
-    ensures isWeekend == old(isWeekend)
+    ensures isWeekend == old(isWeekend) //everything should be unchanged as this method doesnt change anything
     ensures urArea == old(urArea)
     ensures rArea == old(rArea)
     ensures subs == old(subs)
     {
+        //print all of the sets
         print "Subscriptions: ";
         print subs;
         print "\n";
@@ -149,15 +151,6 @@ class {:autocontracts} CarPark{
         print rArea;
         print "\n";
     }
-    /*method LeaveCarPark()
-    requires |urArea| > 0
-    modifies `urArea
-    ensures |urArea| == |old(urArea)| - 1
-    {
-        var leavingCarId : int; //need to make a local var as dafny assume clause only supports local var currently
-        leavingCarId :| leavingCarId in urArea; // taken from lecture 17 finds arbitrary value in the set to remove
-        urArea := urArea - {leavingCarId}; //remove the arbitrary value from the set
-    }*/
 }
 
 method Main(){
@@ -183,14 +176,15 @@ method Main(){
     cp.EnterCarPark(1);
 
     cp.MakeSubscription(8);
+    cp.MakeSubscription(9);
     cp.EnterReserve(8);
+    cp.EnterReserve(9);
     
     //cp.CloseCarPark();
 
     /* WEEKDAY IS FINISHED */
 
     /* TESTING WEEKEND */
-    cp := new CarPark();
 
     print "\n\nWEEKEND PARKING\n\n";
 
